Charge!/src/Open/Stack.v
@@ -1,0 +1,60 @@
+Require Import Rel.
+Require Import FunctionalExtensionality.
+
+Set Implicit Arguments.
+Unset Strict Implicit.
+Set Maximal Implicit Insertion.
+
+Class ValNull := {
+  val    : Type;
+  null   :  val
+}.
+
+Section Defs.
+  Context {A : Type} {H: DecidableEq A}.
+  Context {B : ValNull}.
+
+  Definition stack := A -> val.
+
+  Definition stack_empty : stack := fun x => null.
+
+  Definition stack_add x v s : stack :=
+    fun x' => if dec_eq x' x then v else s x'.
+
+  Lemma stack_lookup_add (s : stack) (x : A) (v : val) :
+      ((stack_add x v s) : stack) x = v.
+  Proof.
+    unfold stack_add. destruct (dec_eq x x); congruence.
+  Qed.
+
+  Lemma stack_lookup_add2 (x y : A) (v : val) (s : stack) (Hneq: x <> y) :
+    (stack_add x v s) y = s y.
+  Proof.
+    unfold stack_add. destruct (dec_eq y x); congruence.
+  Qed.
+
+  Lemma stack_add_same (s: stack) x:
+    stack_add x (s x) s = s.
+  Proof.
+    apply functional_extensionality.
+    intro x'. unfold stack_add. destruct (dec_eq x' x); [rewrite e|];
+    reflexivity.
+  Qed.
+
+  Lemma stack_add_overwrite (s: stack) x v v':
+    stack_add x v (stack_add x v' s) = stack_add x v s.
+  Proof.
+    apply functional_extensionality.
+    intro x'. unfold stack_add. destruct (dec_eq x' x); reflexivity.
+  Qed.
+
+End Defs.
+
+Implicit Arguments stack [[B]].
+Implicit Arguments stack_empty [[B]].
+
+Hint Rewrite @stack_lookup_add
+             @stack_add_same
+             @stack_add_overwrite : stack.
+
+Hint Rewrite @stack_lookup_add2 using solve [auto] : stack.
