Charge!/src/Open/Subst.v
@@ -1,0 +1,224 @@
+Require Import Stack Open Rel.
+Require Import List FunctionalExtensionality.
+
+Set Implicit Arguments.
+Unset Strict Implicit.
+Set Maximal Implicit Insertion.
+
+Fixpoint zip {A} {B} (lst1 : list A) (lst2 : list B) : list (A * B) :=
+  match (lst1, lst2) with
+    | (nil, nil) => nil
+    | (x::xs, nil) => nil
+    | (nil, y::ys) => nil
+    | (x::xs, y::ys) => (x, y) :: zip xs ys
+  end.
+
+Section Subst.
+  Context {A : Type} `{HEq: DecidableEq A}.
+  Context {R : ValNull}.
+
+  Definition subst := A -> @open A R val.
+
+  Definition stack_subst (s: stack A) (sub: subst) : stack A :=
+    fun x => sub x s.
+
+  Definition apply_subst {B}
+          (e : @open A R B) (sub : subst) : @open A R B :=
+    fun s => e (stack_subst s sub).
+
+  Definition substlist := list (A * @expr A R).
+
+  (* The identity substitution *)
+  Definition subst0 : subst := fun x => x/V.
+
+  (* Substitution of one variable *)
+  Definition subst1 e x : subst :=
+    fun x' => if dec_eq x' x then e else x'/V.
+
+  (* Simultaneous substitution of a finite list of variables *)
+  Fixpoint substl_aux (subs: substlist) : subst :=
+    match subs with
+      | nil => subst0
+      | (x,e) :: subs' => fun x' => 
+        if dec_eq x' x then e else substl_aux subs' x'
+    end.
+
+(* Truncating simultaneous substitution of a finite list of variables *)
+  Fixpoint substl_trunc_aux (subs: substlist) : subst :=
+    match subs with
+      | nil => fun _ => empty_open
+      | (x,e) :: subs' => fun x' => 
+        if dec_eq x' x then e else substl_trunc_aux subs' x'
+    end.
+
+  Definition substl es v := substl_aux es v.
+  Definition substl_trunc es v := substl_trunc_aux es v.
+
+End Subst.
+
+(* Binds tighter than function application *)
+(* We have the e at precedence level one less than the precedence of the infix
+   // operator to make parsing work. *)
+
+Notation "g [{ e // x }]" := (apply_subst g (subst1 e x)) (at level 9, e at level 39,
+  format "g [{ e // x }]") : open_scope.
+
+Notation " g '//' es " := (apply_subst g (substl es)) (at level 40) : open_scope.
+
+Notation " g '//!' es " := (apply_subst g (substl_trunc es)) (at level 40) : open_scope.
+
+Section Properties.
+  Context {A : Type} `{Heq: DecidableEq A}.
+  Context {R : ValNull}.
+
+  Lemma open_subst_stack {B} (m: @open A R B) (sub : subst) (s : @stack A R) :
+    (apply_subst m sub) s = m (stack_subst s sub).
+  Proof. reflexivity. Qed.
+
+  Lemma subst0_id B (g: @open A R B) : (apply_subst g (@subst0 A R)) = g.
+  Proof.
+    apply functional_extensionality.
+    intros s; simpl; reflexivity.
+  Qed.
+
+  Lemma subst1_stack (s: @stack A R) e x :
+    stack_subst s (subst1 e x) = stack_add x (e s) s.
+  Proof.
+    apply functional_extensionality; intro x'; simpl.
+    unfold stack_subst, subst1, stack_add. 
+    destruct (dec_eq x' x); reflexivity.
+  Qed.
+
+  Lemma substl_subst1 x e :
+    substl ((x,e)::nil) = subst1 e x.
+  Proof. 
+    reflexivity.
+  Qed.
+  Local Open Scope open_scope.
+  Lemma subst1_stack_add {B} (p : open B) (e : expr) (x : A) (v : val) (s : @stack A R) : 
+    p[{e//x}] (stack_add x v s) = p[{e[{`v//x}]//x}] s.
+  Proof.
+    unfold apply_subst, subst1; simpl.
+    apply f_equal.
+    unfold stack_subst.
+    apply functional_extensionality.
+    intros y.
+    remember (dec_eq y x) as d.
+    destruct d; simpl.
+    apply f_equal.
+    apply functional_extensionality.
+    intros z; simpl.
+    remember (dec_eq z x) as d'.
+    destruct d'; subst.
+    rewrite stack_lookup_add. reflexivity.
+    rewrite stack_lookup_add2. reflexivity.
+    intuition.
+    unfold var_expr.
+    rewrite stack_lookup_add2. reflexivity.
+    intuition.
+  Qed.
+      
+  Lemma stack_add_var (x : A) (s : @stack A R) (v : val) : (x/V) (stack_add x v s) = v.
+  Proof.
+    unfold var_expr. rewrite stack_lookup_add. reflexivity.
+  Qed.
+  
+  Lemma subst1_val (v : val) (e : open val) (x : A) :
+    `v[{e//x}] = `v.
+  Proof.
+    reflexivity.
+  Qed.
+
+  Lemma subst_identity {B} (x : A) (s : @stack A R) (p : open B) :
+    p[{`(s x)//x}] s = p s.
+  Proof.
+    unfold subst1, apply_subst.
+    apply f_equal.
+    unfold stack_subst; simpl.
+    apply functional_extensionality.
+    intros y; simpl.
+    destruct (dec_eq y x); subst; reflexivity.
+  Qed.
+
+  Lemma substl_trunc_notin x' xs es :
+    ~ In x' xs ->
+    substl_trunc (zip xs es) x' = @empty_open _ R.
+  Proof.
+    intro HnotIn. revert es. induction xs as [|x]; intros.
+    + simpl. destruct es; reflexivity.
+    + destruct es as [|e]; [reflexivity|]. simpl. destruct (dec_eq x' x) as [|_].
+      - subst. contradiction HnotIn. simpl. auto.
+      - apply IHxs. auto with datatypes.
+  Qed.
+
+End Properties.
+
+Hint Rewrite @subst0_id : open.
+Hint Rewrite @substl_subst1 : open.
+Hint Rewrite @substl_trunc_notin using assumption : open.
+
+Section MoreLemmas.
+  Context {A : Type} {Heq : DecidableEq A}.
+  Context {R : ValNull}.
+
+  Open Scope open_scope.
+
+  Lemma subst_singleton {B} : 
+    forall x e (P : @open A R B), P[{e//x}] = P // ((x, e)::nil).
+  Proof.
+    reflexivity.
+  Qed.
+
+  Lemma subst_open_expr_nil {B} :
+    forall (e : @open A R B), (e // nil) = e.
+  Proof.
+    reflexivity.
+  Qed.
+
+  Lemma subst_var_cons_eq : 
+    forall (x:A) es (e : expr), ((x/V) // ((x, e)::es)) = e.
+  Proof.
+    intros x es e.
+    apply functional_extensionality; intros s; simpl.
+    unfold var_expr, apply_subst, stack_subst. simpl.
+    case (dec_eq x x); intuition congruence.
+  Qed.
+
+  Lemma subst_var_cons_ineq : forall (x:A) y es (e : expr)
+    (Hneq: x <> y),
+    ((x/V) // ((y, e)::es)) = ((x/V) // es).
+  Proof.
+    intros x y es e Hneq.
+    apply functional_extensionality; intros s.
+    unfold var_expr, apply_subst, stack_subst; simpl.
+    case (dec_eq x y); congruence.
+  Qed.
+
+  Lemma val_expr_substs : forall (v : val) es,
+    ((V_expr v) // es) = (V_expr v).
+  Proof.
+    reflexivity.
+  Qed.
+
+
+  Definition subst_substlist (es fs : @substlist A R) : substlist :=
+    map (fun x => (fst x, (snd x) // fs)) es.
+
+  Lemma subst_combine {B} (e : @open A R B) (es fs : substlist) :
+    (e // es // fs) = (e // ((subst_substlist es fs)++fs)).
+  Proof.
+    apply functional_extensionality; intros s.
+    unfold apply_subst, stack_subst; simpl.
+    f_equal. apply functional_extensionality. intros x.
+    induction es; simpl.
+    + reflexivity.
+    + destruct a; simpl.
+      destruct (dec_eq x a); simpl.
+      * reflexivity.
+      * apply IHes.
+  Qed.
+
+
+Close Scope open_scope.
+
+End MoreLemmas.
